



- 1) Solve the following recurrence using the substitution method - where n is power of 2.

$$T(n) = \begin{cases} 2 & ; \text{ if } n=1 \\ 2T(n/2) + n & ; \text{ if } n > 1. \end{cases}$$

Solⁿ:-

$$T(n) = 2T(n/2) + n \quad \text{--- (1)}$$

put $n=n/2$ in eq (1)

$$\begin{aligned} T(n/2) &= 2T\left(\frac{n/2}{2}\right) + \frac{n}{2} \\ &= 2T\left(\frac{n}{4}\right) + \frac{n}{2} \end{aligned}$$

$$\begin{aligned} T(n) &= 2\left[2T\left(\frac{n}{4}\right) + \frac{n}{2}\right] + n \\ &= 4T\left(\frac{n}{4}\right) + n + n \\ &= 4T\left(\frac{n}{4}\right) + 2n \end{aligned}$$

put $n = n/4$ in eq (1)

$$\begin{aligned} T(n/4) &= 2T\left(\frac{n/4}{2}\right) + \frac{n}{4} \\ &= 2T\left(\frac{n}{8}\right) + \frac{n}{4} \end{aligned}$$

$$= 8 T\left(\frac{n}{8}\right) + n + 2n$$

$$= 8 T\left(\frac{n}{8}\right) + 3n$$

$$= 2^3 T\left(\frac{n}{2^3}\right) + 3n \quad \text{here } i = 3$$

$$\therefore T(n) = 2^i T\left(\frac{n}{2^i}\right) + in \quad \text{for any } \log_2 n \geq i \geq 1$$

$$\text{put } i = \log_2 n \quad \text{where } n = 2^i$$

$$\therefore T(n) = 2^{\log_2 n} T\left(\frac{n}{2^{\log_2 n}}\right) + n \times \log_2 n$$

$$= n T\left(\frac{n}{n}\right) + n \times \log_2 n$$

$$= n(T(1)) + n \times \log_2 n$$

$$\text{But } T(1) = 2$$

$$\therefore T(n) = 2n + n \log_2 n$$

$$\text{Thus } T(n) \in \Theta(n \log_2 n)$$



2) solve the following recurrence when n is power of 2.

merge
sort

$$T(n) = \begin{cases} a & , n=1, a = \text{constant} \\ 2T(n/2) + cn & , n>1, c = \text{constant} \end{cases}$$

n is power of 2. $n = 2^k$.

solⁿ -

$$T(n) = 2T(n/2) + cn \quad \text{--- (1)}$$

put $n = n/2$ in eq (1)

$$T(n/2) = 2T\left(\frac{n/2}{2}\right) + c \frac{n}{2}$$

$$= 2T\left(\frac{n}{4}\right) + c \frac{n}{2}$$

$$T(n) = 2 \left[2T\left(\frac{n}{4}\right) + c \frac{n}{2} \right] + cn$$

$$= 4T\left(\frac{n}{4}\right) + cn + cn$$

$$= 4T\left(\frac{n}{4}\right) + 2cn.$$

put $n = n/4$ in eq. (i)

$$T\left(\frac{n}{4}\right) = 2T\left(\frac{n/4}{2}\right) + c \frac{n}{4}$$

$$= 2T\left(\frac{n}{8}\right) + c \frac{n}{4}.$$

$$\therefore T(n) = 4 \left[2 T\left(\frac{n}{8}\right) + c \frac{n}{4} \right] + 2cn$$

$$= 8 T\left(\frac{n}{8}\right) + \underline{cn + 2cn}$$

$$= 8 T\left(\frac{n}{8}\right) + 3cn \quad \because K=3$$

$$= 2^3 T\left(\frac{n}{2^3}\right) + 3cn$$

$$\therefore T(n) = 2^3 T\left(\frac{2^k}{2^3}\right) + 3cn \quad (n = 2^k)$$

$$= 2^3 T(2^{k-3}) + kcn \quad (k=3)$$

$$\begin{aligned} \therefore T(n) &= 2^k T(1) + kcn & n = 2^k \\ &= n T(1) + kcn & \log n = k \log 2 \\ &= na + cn(\log_2^n) & \therefore k = \log_2^n \\ & & T(1) = a \end{aligned}$$

$\therefore$ it is easy to see that if

$$2^k < n \leq 2^{k+1} \quad \text{then } T(n) \leq T(2^{k+1})$$

$$\therefore T(n) = O(n \log_2^n)$$



3) solve the following recurrence when n is power of 2:

Bubble
sort

$$T(n) = \begin{cases} T(1) & ; \text{if } n=1 \\ T(n/2) + c & ; \text{if } n>1. \end{cases}$$

Solⁿ — $T(n) = T(n/2) + c$ — ①

put $n=n/2$ in eq. ①

$$\therefore T(n/2) = T\left(\frac{n/2}{2}\right) + c.$$

$$T\left(\frac{n}{2}\right) = T\left(\frac{n}{4}\right) + c$$

$$\begin{aligned} \therefore T(n) &= \left[T\left(\frac{n}{4}\right) + c\right] + c \\ &= T\left(\frac{n}{4}\right) + 2c \end{aligned}$$

put $n = n/4$ in eq. ①.

$$\therefore T(n) = T\left(\frac{n}{8}\right) + 3c$$

⋮

$$\therefore T(n) = T\left(\frac{n}{2^i}\right) + ic$$

$$T(n) = T\left(\frac{2}{2^i}\right) + ic$$

$$T(n) = T(1) + ic \quad \text{put } i = \log_2 n$$

$$\begin{aligned} n &= 2^i \\ \log n &= i \log 2 \\ \therefore i &= \log_2 n \end{aligned}$$

$$\therefore T(n) = T(1) + c \log_2^n$$

As $T(1) = \text{constant}$.

$$\therefore T(n) \in \Theta(\log_2^n)$$

$$4) T(n) = \begin{cases} T(1), & n=1 \\ a T(n/b) + f(n), & n>1 \end{cases}$$

where $a = b = \text{constants}$.

$T(1) = \text{known}$.

$\& n = b^k$ (n is a power of b)

solⁿ

$$T(n) = a T(n/b) + f(n) \quad \text{--- (1)}$$

put $n = n/b$ in eq (1)

$$\therefore T(n/b) = a T(n/b^2) + f(n/b)$$

$$T(n/b^2) = a T(n/b^3) + f(n/b^2)$$

$$\therefore T(n) = a \left[a T(n/b^2) + f(n/b) \right] + f(n)$$

$$= a^2 T(n/b^2) + a f(n/b) + f(n)$$

put $n = n/b^2$ in eq. (1) we get.